Moved SET_TAC into pred_setLib; some additions in pred_set and real theories

src/pred_set/src/pred_setLib.sig
@@ -17,4 +17,7 @@ sig
 
   val add_pred_set_compset : computeLib.compset -> unit
 
+  val SET_TAC        : thm list -> tactic
+  val ASM_SET_TAC    : thm list -> tactic
+  val SET_RULE       : term -> thm
 end
