src/pred_set/src/pred_setScript.sml
@@ -826,6 +826,14 @@ val DISJOINT_SUBSET = Q.store_thm
                EXTENSION] THEN
   PROVE_TAC []);
 
+val SUBSET_DISJOINT = store_thm
+  ("SUBSET_DISJOINT",
+  ``!s t u v. DISJOINT s t /\ u SUBSET s /\ v SUBSET t ==> DISJOINT u v``,
+    RW_TAC std_ss [DISJOINT_ALT]
+ >> `x IN s` by PROVE_TAC [SUBSET_DEF]
+ >> CCONTR_TAC >> fs []
+ >> `x IN t` by PROVE_TAC [SUBSET_DEF]
+ >> RES_TAC);
 
 (* ===================================================================== *)
 (* Set difference                                                        *)
@@ -930,7 +938,7 @@ val DISJOINT_DIFF = store_thm (* from util_prob *)
 
 val DISJOINT_DIFFS = store_thm (* from util_prob *)
   ("DISJOINT_DIFFS",
-   ``!f m n.
+   ``!f g m n.
        (!n. f n SUBSET f (SUC n)) /\
        (!n. g n = f (SUC n) DIFF f n) /\ ~(m = n) ==>
        DISJOINT (g m) (g n)``,
@@ -1612,6 +1620,17 @@ val IMAGE_EMPTY =
       REWRITE_TAC[EXTENSION,IN_IMAGE,NOT_IN_EMPTY]);
 val _ = export_rewrites ["IMAGE_EMPTY"]
 
+val IMAGE_EMPTY_FUN = store_thm
+  ("IMAGE_EMPTY_FUN",
+  ``!s. s <> EMPTY ==> (IMAGE (\i. EMPTY) s = {EMPTY})``,
+    rpt STRIP_TAC
+ >> RW_TAC std_ss [EXTENSION, IN_IMAGE, IN_SING, NOT_IN_EMPTY]
+ >> EQ_TAC >> rpt STRIP_TAC
+ >> Q.EXISTS_TAC `CHOICE s`
+ >> ASM_REWRITE_TAC []
+ >> MATCH_MP_TAC CHOICE_DEF
+ >> ASM_REWRITE_TAC []);
+
 val IMAGE_ID =
     store_thm
     ("IMAGE_ID",
@@ -1741,6 +1760,11 @@ val EXISTS_IN_IMAGE = store_thm
   ``!P f s. (?y. y IN IMAGE f s /\ P y) <=> ?x. x IN s /\ P(f x)``,
     REWRITE_TAC [IN_IMAGE] THEN PROVE_TAC []);
 
+val IMAGE_SING = store_thm (* from measureTheory *)
+  ("IMAGE_SING", ``!f x. IMAGE f {x} = {f x}``,
+    RW_TAC std_ss [EXTENSION,IN_SING,IN_IMAGE] >> METIS_TAC []);
+val _ = export_rewrites ["IMAGE_SING"];
+
 (* ===================================================================== *)
 (* Injective functions on a set.                                         *)
 (* ===================================================================== *)
@@ -1785,14 +1809,14 @@ val INJ_EMPTY =
      REPEAT (STRIP_TAC ORELSE EQ_TAC) THEN RES_TAC);
 
 val INJ_DELETE = Q.store_thm
-("INJ_DELETE",
- `!s t f. INJ f s t ==> !e. e IN s ==> INJ f (s DELETE e) (t DELETE (f e))`,
-RW_TAC bool_ss [INJ_DEF, DELETE_DEF] THENL
-[`~(e = x)` by FULL_SIMP_TAC bool_ss
+  ("INJ_DELETE",
+   `!f s t. INJ f s t ==> !e. e IN s ==> INJ f (s DELETE e) (t DELETE (f e))`,
+  RW_TAC bool_ss [INJ_DEF, DELETE_DEF] THENL
+  [`~(e = x)` by FULL_SIMP_TAC bool_ss
                  [DIFF_DEF,DIFF_INSERT, DIFF_EMPTY, IN_DELETE] THEN
   FULL_SIMP_TAC bool_ss [DIFF_DEF,DIFF_INSERT, DIFF_EMPTY, IN_DELETE] THEN
   METIS_TAC [],
-METIS_TAC [IN_DIFF]]);
+  METIS_TAC [IN_DIFF]]);
 
 Theorem INJ_INSERT:
   !f x s t. INJ f (x INSERT s) t <=>
@@ -1803,9 +1827,11 @@ Proof
 QED
 
 val INJ_EXTEND = Q.store_thm(
-  "INJ_EXTEND",
-  `INJ b s t /\ x NOTIN s /\ y NOTIN t ==>
+   "INJ_EXTEND",
+  `!b s t x y.
+    INJ b s t /\ x NOTIN s /\ y NOTIN t ==>
     INJ ((x =+ y) b) (x INSERT s) (y INSERT t)`,
+  rpt GEN_TAC \\
   fs[INJ_DEF,combinTheory.APPLY_UPDATE_THM] >> METIS_TAC []);
 
 val INJ_SUBSET = store_thm(
@@ -1814,15 +1840,17 @@ val INJ_SUBSET = store_thm(
 SRW_TAC[][INJ_DEF,SUBSET_DEF])
 
 val INJ_IMAGE = Q.store_thm ("INJ_IMAGE",
-  `INJ f s t ==> INJ f s (IMAGE f s)`,
+  `!f s t. INJ f s t ==> INJ f s (IMAGE f s)`,
+  REPEAT GEN_TAC THEN
   REWRITE_TAC [INJ_DEF, IN_IMAGE] THEN
   REPEAT DISCH_TAC THEN ASM_REWRITE_TAC [] THEN
-  REPEAT STRIP_TAC THEN Q.EXISTS_TAC `x` THEN ASM_REWRITE_TAC [])  ;
+  REPEAT STRIP_TAC THEN Q.EXISTS_TAC `x` THEN ASM_REWRITE_TAC []);
 
 val INJ_IMAGE_SUBSET = Q.store_thm ("INJ_IMAGE_SUBSET",
-  `INJ f s t ==> IMAGE f s SUBSET t`,
+  `!f s t. INJ f s t ==> IMAGE f s SUBSET t`,
+  REPEAT GEN_TAC THEN
   REWRITE_TAC [INJ_DEF, SUBSET_DEF, IN_IMAGE] THEN
-  REPEAT STRIP_TAC THEN BasicProvers.VAR_EQ_TAC THEN RES_TAC) ;
+  REPEAT STRIP_TAC THEN BasicProvers.VAR_EQ_TAC THEN RES_TAC);
 
 (* ===================================================================== *)
 (* Surjective functions on a set.                                        *)
@@ -2601,6 +2629,7 @@ val FINITE_SING =
      GEN_TAC THEN MP_TAC FINITE_EMPTY THEN
      SUBST1_TAC (SYM (SPEC (“x:'a”) SING_DELETE)) THEN
      DISCH_TAC THEN IMP_RES_THEN MATCH_ACCEPT_TAC FINITE_INSERT);
+val _ = export_rewrites ["FINITE_SING"]
 
 val SING_FINITE =
     store_thm
@@ -3289,14 +3318,31 @@ val CARD_COUNT = store_thm
     THEN CONV_TAC Arith.ARITH_CONV]);
 val _ = export_rewrites ["CARD_COUNT"]
 
-val COUNT_11 = store_thm(
-  "COUNT_11",
-  ``(count n1 = count n2) <=> (n1 = n2)``,
-  SRW_TAC [][EQ_IMP_THM, EXTENSION] THEN
-  METIS_TAC [numLib.ARITH_PROVE ``x:num < y <=> ~(y <= x)``,
-             arithmeticTheory.LESS_EQ_REFL,
-             arithmeticTheory.LESS_EQUAL_ANTISYM]);
-val _ = export_rewrites ["COUNT_11"]
+val COUNT_11 = store_thm
+  ("COUNT_11", ``(count n1 = count n2) <=> (n1 = n2)``,
+    SRW_TAC [] [EQ_IMP_THM, EXTENSION]
+ >> METIS_TAC [numLib.ARITH_PROVE ``x:num < y <=> ~(y <= x)``,
+               LESS_EQ_REFL, LESS_EQUAL_ANTISYM]);
+val _ = export_rewrites ["COUNT_11"];
+
+val COUNT_DELETE = store_thm (* added by measureTheory *)
+  ("COUNT_DELETE", ``!n. count n DELETE n = count n``,
+    SRW_TAC [] [EQ_IMP_THM, EXTENSION]);
+val _ = export_rewrites ["COUNT_DELETE"];
+
+val COUNT_MONO = store_thm (* added by extrealTheory *)
+  ("COUNT_MONO", ``!m n. m <= n ==> (count m) SUBSET (count n)``,
+    SRW_TAC [] [count_def, SUBSET_DEF, GSPECIFICATION]
+ >> RW_TAC arith_ss []);
+
+val COUNT_NOT_EMPTY = store_thm (* added by probabilityTheory *)
+  ("COUNT_NOT_EMPTY", ``!n. 0 < n <=> count n <> {}``,
+    RW_TAC arith_ss [Once EXTENSION, IN_COUNT, NOT_IN_EMPTY]
+ >> EQ_TAC >> STRIP_TAC
+ >- (Q.EXISTS_TAC `0` >> ASM_REWRITE_TAC [])
+ >> `0 <= x` by RW_TAC arith_ss []
+ >> MATCH_MP_TAC LESS_EQ_LESS_TRANS
+ >> Q.EXISTS_TAC `x` >> ASM_REWRITE_TAC []);
 
 (* =====================================================================*)
 (* Infiniteness                                                         *)
@@ -3782,6 +3828,11 @@ Proof
   PROVE_TAC []
 QED
 
+val SUBSET_BIGUNION = Q.store_thm
+  ("SUBSET_BIGUNION", `!s P. s IN P ==> s SUBSET (BIGUNION P)`,
+    RW_TAC std_ss [SUBSET_DEF, IN_BIGUNION]
+ >> Q.EXISTS_TAC `s` >> ASM_REWRITE_TAC []);
+
 val BIGUNION_IMAGE_UNIV = store_thm (* from util_prob *)
   ("BIGUNION_IMAGE_UNIV",
    ``!f N.
@@ -4239,6 +4290,10 @@ val COMPL_UNION = Q.store_thm(
 "COMPL_UNION",
 `COMPL (s UNION t) = COMPL s INTER COMPL t`,
 SRW_TAC [][EXTENSION,COMPL_DEF]);
+
+val DIFF_INTER_COMPL = store_thm
+  ("DIFF_INTER_COMPL", ``!s t. s DIFF t = s INTER (COMPL t)``,
+    RW_TAC std_ss [EXTENSION, IN_DIFF, IN_INTER, IN_COMPL]);
 
 (*---------------------------------------------------------------------------
     A "fold"-like operation for sets.
@@ -5005,6 +5060,11 @@ val POW_EMPTY = store_thm("POW_EMPTY",
   SRW_TAC[][EXTENSION,IN_POW] THEN
   METIS_TAC[EMPTY_SUBSET])
 val _ = export_rewrites["POW_EMPTY"]
+
+val EMPTY_IN_POW = store_thm
+  ("EMPTY_IN_POW", ``!s. {} IN POW s``,
+    RW_TAC std_ss [IN_POW, EMPTY_SUBSET]);
+val _ = export_rewrites["EMPTY_IN_POW"];
 
 (*---------------------------------------------------------------------------*)
 (* Recursion equations for POW                                               *)
@@ -5891,22 +5951,22 @@ SIMP_TAC bool_ss [IN_BIGUNION, IN_IMAGE,
 METIS_TAC[]);
 
 
-val SUBSET_DIFF = store_thm("SUBSET_DIFF",
-``!s1 s2 s3.
-(s1 SUBSET (s2 DIFF s3)) =
-((s1 SUBSET s2) /\ (DISJOINT s1 s3))``,
+val SUBSET_DIFF = store_thm ("SUBSET_DIFF",
+  ``!s1 s2 s3. (s1 SUBSET (s2 DIFF s3)) <=> s1 SUBSET s2 /\ DISJOINT s1 s3``,
+    SIMP_TAC bool_ss [SUBSET_DEF, IN_DIFF, DISJOINT_DEF, EXTENSION, IN_INTER,
+                      NOT_IN_EMPTY]
+ >> METIS_TAC []);
 
-SIMP_TAC bool_ss [SUBSET_DEF, IN_DIFF, DISJOINT_DEF, EXTENSION, IN_INTER, NOT_IN_EMPTY] THEN
-METIS_TAC[])
+val SUBSET_DIFF_DISJOINT = store_thm (* added by measureTheory *)
+  ("SUBSET_DIFF_DISJOINT",
+  ``!s1 s2 s3. (s1 SUBSET (s2 DIFF s3)) ==> DISJOINT s1 s3``,
+    PROVE_TAC [SUBSET_DIFF]);
 
 val INTER_SUBSET_EQN = store_thm ("INTER_SUBSET_EQN",
-
-``((A INTER B = A) = (A SUBSET B)) /\
-  ((A INTER B = B) = (B SUBSET A))``,
-
-SIMP_TAC bool_ss [EXTENSION, IN_INTER, SUBSET_DEF] THEN
-METIS_TAC[]);
-
+  ``((A INTER B = A) = (A SUBSET B)) /\
+    ((A INTER B = B) = (B SUBSET A))``,
+    SIMP_TAC bool_ss [EXTENSION, IN_INTER, SUBSET_DEF]
+ >> METIS_TAC []);
 
 Theorem PSUBSET_SING:
   !s x. x PSUBSET {s} <=> (x = EMPTY)
